Checkpoint progress on proofmode that works well with IntoVal

new/golang/theory/pure_proofmode.v
@@ -1,5 +1,6 @@
 From Perennial.program_logic Require Export weakestpre.
 From Perennial.goose_lang Require Export lang lifting.
+From Perennial.Helpers Require Export ipm.
 From iris.proofmode Require Import coq_tactics.
 From New.golang.theory Require Export typing.
 From Ltac2 Require Import Ltac2.
@@ -17,20 +18,19 @@ Class PureWp `{ffi_sem: ffi_semantics} `{!ffi_interp ffi} `{!gooseGlobalGS Σ, !
 Global Hint Mode PureWp - - - - - - - - ! - : typeclass_instances.
 
 Lemma tac_wp_pure_wp `{ffi_sem: ffi_semantics} `{!ffi_interp ffi} `{!gooseGlobalGS Σ, !gooseLocalGS Σ}
-      K e1 Δ Δ' s E (e2 : expr) φ Φ :
-  PureWp φ e1 e2 →
+      K e1 {e2 φ} (Hwp:PureWp φ e1 e2) Δ Δ' s E Φ :
   φ →
   MaybeIntoLaterNEnvs 1 Δ Δ' →
   envs_entails Δ' (WP (fill K e2) @ s; E {{ Φ }}) →
   envs_entails Δ (WP (fill K e1) @ s; E {{ Φ }}).
 Proof.
-  rewrite envs_entails_unseal=> Hstep ?? HΔ'. rewrite into_laterN_env_sound /=.
-  rewrite HΔ'. iIntros "H". by iApply Hstep.
+  rewrite envs_entails_unseal=> ?? HΔ'. rewrite into_laterN_env_sound /=.
+  rewrite HΔ'. iIntros "H". by iApply Hwp.
 Qed.
 
 (* Now a few lemmas to help establish PureWp in other ways. *)
 Lemma pure_wp_val
-  `{ffi_sem: ffi_semantics} `{!ffi_interp ffi} `{!heapGS Σ}
+  `{ffi_sem: ffi_semantics} `{!ffi_interp ffi} `{!gooseGlobalGS Σ, !gooseLocalGS Σ}
   φ e v' :
   (∀ stk E Φ (H : φ), ▷ Φ v' -∗ WP e @ stk ; E {{ Φ }}) →
   PureWp φ e (Val v').
@@ -41,7 +41,7 @@ Proof.
 Qed.
 
 Lemma pure_exec_pure_wp n
-  `{ffi_sem: ffi_semantics} `{!ffi_interp ffi} `{!heapGS Σ} {φ e e'} :
+  `{ffi_sem: ffi_semantics} `{!ffi_interp ffi} `{!gooseGlobalGS Σ, !gooseLocalGS Σ} {φ e e'} :
   PureExec φ (S n) e e' → PureWp φ e e'.
 Proof.
   intros ??????.
@@ -55,7 +55,7 @@ End classes.
 
 (** Some basic, primitive instances. Adapted to use `IntoVal`. *)
 Section instances.
-Context `{ffi_sem: ffi_semantics} `{!ffi_interp ffi} `{!heapGS Σ}.
+Context `{ffi_sem: ffi_semantics} `{!ffi_interp ffi} `{!gooseGlobalGS Σ, !gooseLocalGS Σ}.
 
 Global Instance wp_injl (v : val) : PureWp True (InjL v) (InjLV v).
 Proof. apply (pure_exec_pure_wp O). solve_pure_exec. Qed.
@@ -90,13 +90,16 @@ Proof. apply (pure_exec_pure_wp O). solve_pure_exec. Qed.
 Global Instance wp_total_le (v1 v2 : val) : PureWp True (TotalLe v1 v2) #(val_le v1 v2).
 Proof. apply (pure_exec_pure_wp O). rewrite to_val_unseal. solve_pure_exec. Qed.
 
-Global Instance wp_eq `{!IntoVal V} `{!IntoValTyped V t} `{!IntoValTypedComparable V t} (v1 v2 : V) :
-  PureWp True (BinOp EqOp #v1 #v2) #(bool_decide (v1 = v2)).
+Global Instance wp_eq `{!IntoVal V} `{!IntoValTyped V t} (v1 v2 : V) :
+  PureWp (is_comparable_go_type t = true) (BinOp EqOp #v1 #v2) #(bool_decide (v1 = v2)) | 0.
 Proof.
-  pose proof (conj (to_val_is_comparable v1) (to_val_is_comparable v2)).
+  apply (pure_exec_pure_wp O).
+  intros Hcomp.
+  pose proof (conj (to_val_is_comparable v1 ltac:(done)) (to_val_is_comparable v2 ltac:(done))).
+  revert Hcomp.
   rewrite to_val_unseal in H.
   cut (bin_op_eval EqOp (to_val_def v1) (to_val_def v2) = Some $ LitV $ LitBool $ bool_decide (v1 = v2)).
-  { rewrite to_val_unseal. intros. apply (pure_exec_pure_wp O). solve_pure_exec. }
+  { rewrite to_val_unseal. intros ?. solve_pure_exec. }
   rewrite /bin_op_eval /bin_op_eval_eq /=.
   rewrite decide_True //.
   destruct (decide (v1 = v2)) eqn:Hx.
@@ -190,7 +193,7 @@ Proof. rewrite to_val_unseal. apply (pure_exec_pure_wp O). solve_pure_exec. Qed.
 
 (* w64 binop instance *)
 Global Instance wp_w64_binop op (v1 v2 : w64) (v : w64) :
-  PureWp (op ≠ EqOp ∧ bin_op_eval_word op v1 v2 = Some v) (BinOp op #v1 #v2)%E #v.
+  PureWp (op ≠ EqOp ∧ bin_op_eval_word op v1 v2 = Some v) (BinOp op #v1 #v2)%E #v | 1.
 Proof.
   rewrite to_val_unseal. apply (pure_exec_pure_wp O). solve_pure_exec; destruct H as [Hneq Hword].
   - rewrite /bin_op_eval Hword decide_False // union_Some_l /=. Transitions.monad_simpl.
@@ -198,7 +201,7 @@ Proof.
 Qed.
 
 Global Instance wp_w32_binop op (v1 v2 : w32) (v : w32) :
-  PureWp (op ≠ EqOp ∧ bin_op_eval_word op v1 v2 = Some v) (BinOp op #v1 #v2)%E #v.
+  PureWp (op ≠ EqOp ∧ bin_op_eval_word op v1 v2 = Some v) (BinOp op #v1 #v2)%E #v | 1.
 Proof.
   rewrite to_val_unseal. apply (pure_exec_pure_wp O). solve_pure_exec; destruct H as [Hneq Hword].
   - rewrite /bin_op_eval Hword decide_False // union_Some_l /=. Transitions.monad_simpl.
@@ -206,7 +209,7 @@ Proof.
 Qed.
 
 Global Instance wp_w8_binop op (v1 v2 : w8) (v : w8) :
-  PureWp (op ≠ EqOp ∧ bin_op_eval_word op v1 v2 = Some v) (BinOp op #v1 #v2)%E #v.
+  PureWp (op ≠ EqOp ∧ bin_op_eval_word op v1 v2 = Some v) (BinOp op #v1 #v2)%E #v | 1.
 Proof.
   rewrite to_val_unseal. apply (pure_exec_pure_wp O). solve_pure_exec; destruct H as [Hneq Hword].
   - rewrite /bin_op_eval Hword decide_False // union_Some_l /=. Transitions.monad_simpl.
@@ -214,7 +217,7 @@ Proof.
 Qed.
 
 Global Instance wp_w8_w64_binop op (v1 : w8) (v2 : w64) (v : w8) :
-  PureWp (bin_op_eval_shift op v1 (W8 (uint.Z v2)) = Some v) (BinOp op #v1 #v2) #v.
+  PureWp (bin_op_eval_shift op v1 (W8 (uint.Z v2)) = Some v) (BinOp op #v1 #v2) #v | 1.
 Proof.
   rewrite to_val_unseal. apply (pure_exec_pure_wp O).
   rewrite /bin_op_eval_shift /=.
@@ -223,7 +226,7 @@ Proof.
 Qed.
 
 Global Instance wp_w8_w32_binop op (v1 : w8) (v2 : w32) (v : w8) :
-  PureWp (bin_op_eval_shift op v1 (W8 (uint.Z v2)) = Some v) (BinOp op #v1 #v2) #v.
+  PureWp (bin_op_eval_shift op v1 (W8 (uint.Z v2)) = Some v) (BinOp op #v1 #v2) #v | 1.
 Proof.
   rewrite to_val_unseal. apply (pure_exec_pure_wp O).
   intros H. destruct op; simpl in H; try by exfalso.
@@ -231,7 +234,7 @@ Proof.
 Qed.
 
 Global Instance wp_w32_w64_binop op (v1 : w32) (v2 : w64) (v : w32) :
-  PureWp (bin_op_eval_shift op v1 (W32 (uint.Z v2)) = Some v) (BinOp op #v1 #v2) #v.
+  PureWp (bin_op_eval_shift op v1 (W32 (uint.Z v2)) = Some v) (BinOp op #v1 #v2) #v | 1.
 Proof.
   rewrite to_val_unseal. apply (pure_exec_pure_wp O).
   intros H. destruct op; simpl in H; try by exfalso.
@@ -239,7 +242,7 @@ Proof.
 Qed.
 
 Global Instance wp_w32_w8_binop op (v1 : w32) (v2 : w8) (v : w32) :
-  PureWp (bin_op_eval_shift op v1 (W32 (uint.Z v2)) = Some v) (BinOp op #v1 #v2) #v.
+  PureWp (bin_op_eval_shift op v1 (W32 (uint.Z v2)) = Some v) (BinOp op #v1 #v2) #v | 1.
 Proof.
   rewrite to_val_unseal. apply (pure_exec_pure_wp O).
   intros H. destruct op; simpl in H; try by exfalso.
@@ -247,7 +250,7 @@ Proof.
 Qed.
 
 Global Instance wp_w64_w8_binop op (v1 : w64) (v2 : w8) (v : w64) :
-  PureWp (bin_op_eval_shift op v1 (W64 (uint.Z v2)) = Some v) (BinOp op #v1 #v2) #v.
+  PureWp (bin_op_eval_shift op v1 (W64 (uint.Z v2)) = Some v) (BinOp op #v1 #v2) #v | 1.
 Proof.
   rewrite to_val_unseal. apply (pure_exec_pure_wp O).
   intros H. destruct op; simpl in H; try by exfalso.
@@ -255,7 +258,7 @@ Proof.
 Qed.
 
 Global Instance wp_w64_w32_binop op (v1 : w64) (v2 : w32) (v : w64) :
-  PureWp (bin_op_eval_shift op v1 (W64 (uint.Z v2)) = Some v) (BinOp op #v1 #v2) #v.
+  PureWp (bin_op_eval_shift op v1 (W64 (uint.Z v2)) = Some v) (BinOp op #v1 #v2) #v | 1.
 Proof.
   rewrite to_val_unseal. apply (pure_exec_pure_wp O).
   intros H. destruct op; simpl in H; try by exfalso.
@@ -264,7 +267,7 @@ Qed.
 
 (* bool binop *)
 Global Instance wp_bool_binop op (v1 v2 v : bool) :
-  PureWp (op ≠ EqOp ∧ bin_op_eval_bool op v1 v2 = Some v) (BinOp op #v1 #v2) #v.
+  PureWp (op ≠ EqOp ∧ bin_op_eval_bool op v1 v2 = Some v) (BinOp op #v1 #v2) #v | 1.
 Proof.
   rewrite to_val_unseal. apply (pure_exec_pure_wp O).
   case => ?. solve_pure_exec.
@@ -273,7 +276,7 @@ Proof.
 Qed.
 
 Global Instance wp_string_binop op (v1 v2 v : string) :
-  PureWp (op ≠ EqOp ∧ bin_op_eval_string op v1 v2 = Some v) (BinOp op #v1 #v2) #v.
+  PureWp (op ≠ EqOp ∧ bin_op_eval_string op v1 v2 = Some v) (BinOp op #v1 #v2) #v | 1.
 Proof.
   rewrite to_val_unseal. apply (pure_exec_pure_wp O).
   case => ?. solve_pure_exec.
@@ -311,8 +314,145 @@ Proof.
   - rewrite /bin_op_eval /= H /= in H1. Transitions.monad_inv. done.
 Qed.
 
-(* TODO: beta *)
+(* XXX: making this an instance results in this fact getting used even in places
+  where the RecV is under a definition. Making it an explicit [Hint Extern]
+  below alleviates this problem, and only applies [wp_call] when the goal
+  expression is syntactically a [RecV]. *)
+Definition wp_call (v2 : val) f x e :
+  PureWp True (App (rec: f x := e)%V v2) (subst' x v2 (subst' f (rec: f x := e)%V e)).
+Proof. apply (pure_exec_pure_wp O). solve_pure_exec. Qed.
 
 End instances.
 
+Global Hint Extern 0 (PureWp _ (App (Val (RecV _ _ _)) _) _) => simple apply wp_call : typeclass_instances.
+
+Section lemmas.
+Lemma tac_wp_bind `{ffi_sem: ffi_semantics} `{!ffi_interp ffi} `{!gooseLocalGS Σ, !gooseGlobalGS Σ}
+    K e Δ s E Φ f :
+  f = (λ e, fill K e) → (* as an eta expanded hypothesis so that the `wp_bind`
+                           tactic can `simpl` the RHS to get a concrete function
+                           f which results in a nice looking output without
+                           `fill K` appearing. *)
+  envs_entails Δ (WP e @ s; E {{ v, WP f (Val v) @ s; E {{ Φ }} }})%I →
+  envs_entails Δ (WP fill K e @ s; E {{ Φ }}).
+Proof. rewrite envs_entails_unseal=> -> ->. by apply: wp_bind. Qed.
+
+Lemma tac_wp_rec `{ffi_sem: ffi_semantics} `{!ffi_interp ffi} `{!gooseGlobalGS Σ, !gooseLocalGS Σ}
+      K v1 v2 {f x e} {Hwp:TCEq v1 (rec: f x := e)%V} Δ Δ' s E Φ :
+  MaybeIntoLaterNEnvs 1 Δ Δ' →
+  envs_entails Δ' (WP (fill K (subst' x v2 (subst' f v1 e))) @ s; E {{ Φ }}) →
+  envs_entails Δ (WP (fill K (App v1 v2)) @ s; E {{ Φ }}).
+Proof.
+  rewrite envs_entails_unseal=> ? HΔ'. rewrite into_laterN_env_sound /=.
+  rewrite HΔ'. iIntros "H". rewrite TCEq_eq in Hwp. rewrite Hwp.
+  by iApply wp_call.
+Qed.
+
+End lemmas.
+
 (** Tactics *)
+Ltac2 walk_expr (e : constr) (f : constr -> constr -> 'a) : 'a :=
+  let rec walk_ctx (e : constr) (k : constr) :=
+    lazy_match! e with | Val _ => Control.backtrack_tactic_failure "walk_expr: reached a val" | _ => () end;
+    match! e with
+    | _ => f e k
+    | fill ?k' ?e                     => walk_ctx e '($k ++ $k')
+    | App ?e1 (Val ?v)                => walk_ctx e1 '(@AppLCtx _ $v :: $k)
+    | App ?e1 ?e2                     => walk_ctx e2 '(@AppRCtx _ $e1 :: $k)
+    | UnOp ?op ?e                     => walk_ctx e '(@UnOpCtx _ $op :: $k)
+    | BinOp ?op (Val ?v) ?e           => walk_ctx e '(@BinOpRCtx _ $op $v :: $k)
+    | BinOp ?op ?e1 ?e2               => walk_ctx e1 '(@BinOpLCtx _ $op $e2 :: $k)
+    | If ?e0 ?e1 ?e2                  => walk_ctx e0 '(IfCtx $e1 $e2 :: $k)
+    | Pair (Val ?v) ?e                => walk_ctx e '(PairRCtx $v :: $k)
+    | Pair ?e1 ?e2                    => walk_ctx e1 '(PairLCtx $e2 :: $k)
+    | Fst ?e                          => walk_ctx e '(@FstCtx _ :: $k)
+    | Snd ?e                          => walk_ctx e '(@SndCtx _ :: $k)
+    | InjL ?e                         => walk_ctx e '(@InjLCtx _ :: $k)
+    | InjR ?e                         => walk_ctx e '(@InjRCtx _ :: $k)
+    | Case ?e0 ?e1 ?e2                => walk_ctx e0 '(CaseCtx $e1 $e2 :: $k)
+    | Primitive2 ?op (Val ?v) ?e      => walk_ctx e '(@Primitive2RCtx _ $op $v :: $k)
+    | Primitive2 ?op ?e1 ?e2          => walk_ctx e1 '(@Primitive2LCtx _ $op $e2 :: $k)
+    | Primitive1 ?op ?e               => walk_ctx e '(@Primitive1Ctx _ $op :: $k)
+    | ExternalOp ?op ?e               => walk_ctx e '(@ExternalOpCtx _ $op :: $k)
+    | CmpXchg (Val ?v0) (Val ?v1) ?e2 => walk_ctx e2 '(CmpXchgRCtx $v0 $v1 :: $k)
+    | CmpXchg (Val ?v0) ?e1 ?e2       => walk_ctx e1 '(CmpXchgMCtx $v0 $e2 :: $k)
+    | CmpXchg ?e0 ?e1 ?e2             => walk_ctx e0 '(CmpXchgLCtx $e1 $e2 :: $k)
+    | ResolveProph (Val ?v) ?e        => walk_ctx e '(@ResolveProphRCtx _ $v :: $k)
+    | ResolveProph ?e1 ?e2            => walk_ctx e1 '(@ResolveProphLCtx _ $e2 :: $k)
+    end
+  in (walk_ctx e) '(@nil ectx_item)
+.
+
+Ltac2 wp_pure () :=
+  lazy_match! goal with
+  | [ |- envs_entails _ (wp _  _ ?e _) ] =>
+      orelse (fun () => walk_expr e (fun e k =>
+                                    (* This looks for an instance before eapply to make to fail fast. *)
+                                    let pure_wp := '(ltac:(tc_solve) : PureWp _ $e _) in
+                                    eapply (tac_wp_pure_wp $k $e $pure_wp) >
+                                      [ltac1:(done)|ltac1:(tc_solve)|
+                                        ltac1:(reduction.pm_prettify; simpl subst'; simpl fill)]
+                       )
+        )
+        (fun _ => Control.backtrack_tactic_failure "wp_pure: could not find a head subexpression with a known next step")
+  | [ |-  _ ] => Control.backtrack_tactic_failure "wp_pure: current proof is not a WP"
+  end.
+Tactic Notation "wp_pure" := ltac2:(wp_pure ()).
+Tactic Notation "wp_pures" := repeat wp_pure.
+
+Ltac2 wp_call () :=
+  lazy_match! goal with
+  | [ |- envs_entails _ (wp _  _ ?e _) ] =>
+      orelse (fun () => walk_expr e (fun e k =>
+                                    Std.unify e '(App _ _);
+                                    eapply (tac_wp_rec $k) >
+                                      [ltac1:(tc_solve) | ltac1:(tc_solve)|
+                                        ltac1:(reduction.pm_prettify; simpl subst'; simpl fill)]
+                       )
+        )
+        (fun _ => Control.backtrack_tactic_failure "wp_call: could not find a function call expression at the head")
+  | [ |-  _ ] => Control.backtrack_tactic_failure "wp_call: current proof is not a WP"
+  end.
+Tactic Notation "wp_call" := ltac2:(wp_call ()); wp_pures.
+
+Ltac2 wp_bind_filter (filter_tac : constr -> unit) : unit :=
+  lazy_match! goal with
+  | [ |- envs_entails _ (wp _  _ ?e _) ] =>
+      walk_expr e (fun e' k => filter_tac e';
+                            eapply (tac_wp_bind $k $e') >
+                              [simpl; reflexivity|ltac1:(reduction.pm_prettify)])
+  end.
+
+(*
+Ltac2 wp_pure :=
+  lazy_match! goal with
+  | [ |- envs_entails Δ (wp ?s ?emask ?e ?q) ] =>
+      orelse (walk_expr e (fun e k =>
+                             (* see if there is an instance *)
+                             let pure_wp := '(ltac:(tc_solve) : PureWp _ $e _) in
+                             eapply (tac_wp_pure_wp k e pure_wp);
+                )
+        )
+        (Control.backtrack_tactic_failure "wp_pure: could not find a head subexpression with a known next step")
+.
+
+Definition x : expr := (App (#false + #false) (#true - #true)).
+Fail Ltac2 Eval (walk_expr '(App (#false + #false) (#true - #true)))
+  (fun e k => fail; Control.assert_true false).
+
+From Ltac2 Require Import Message.
+Ltac2 msg x := print (of_string x).
+Lemma y : True.
+Proof.
+  Proof Mode "Ltac2".
+  Fail (walk_expr '(App (#false + #false) (#true - #true)))
+    (fun e k => Message.print (of_constr '($e, $k)); fail).
+  lazy_match! 'True with
+  | True => msg "branch 1"; fail
+  | _ => msg "branch 2"
+  end.
+
+Ltac2 Eval lazy_match! 'True with
+| True => msg "branch 1"; fail
+| _ => msg "branch 2"
+end. *)
